Phi_Examples/PhiEx_BiTree.thy
@@ -206,7 +206,7 @@ lemma sorted1_inorder_map_tree[iff]:
 
 
 
-  
+   
 \<phi>type_def Bin_Search_Tree :: \<open>logaddr \<Rightarrow> TY \<Rightarrow> TY \<Rightarrow> (VAL, 'k::linorder) \<phi> \<Rightarrow> (VAL, 'v) \<phi> \<Rightarrow> (fiction, 'k \<rightharpoonup> 'v) \<phi>\<close>
   where \<open>f \<Ztypecolon> Bin_Search_Tree addr TY\<^sub>K TY\<^sub>V K V \<equiv> tree \<Ztypecolon> BiTree addr (\<s>\<t>\<r>\<u>\<c>\<t> {k: TY\<^sub>K, v: TY\<^sub>V}) \<lbrace> k: K, v: V \<rbrace>
                                        \<s>\<u>\<b>\<j> tree. f = lookup_tree tree \<and> sorted1(inorder tree)\<close>
