Phi_Semantics/PhiSem_Mem_C.thy
@@ -196,7 +196,7 @@ ML \<open>@{term \<open>\<m>\<e>\<m>[addr] (MAKE (n \<odiv> \<m>\<e>\<m>-\<c>\<o
 
 paragraph \<open>Slice\<close>
 
-consts Slice_synt :: \<open>nat \<Rightarrow> nat \<Rightarrow> (mem_fic,'a) \<phi> \<Rightarrow> (mem_fic, 'a list) \<phi>\<close> ("\<s>\<l>\<i>\<c>\<e>[_, _] _" [10,10,911] 910)
+consts Slice_synt :: \<open>nat \<Rightarrow> nat \<Rightarrow> (mem_fic,'a) \<phi> \<Rightarrow> (mem_fic, 'a list) \<phi>\<close> ("\<s>\<l>\<i>\<c>\<e>[_, _] _" [10,10,910] 911)
 
 translations "\<s>\<l>\<i>\<c>\<e>[start, len] T" == "\<big_ast>\<^sub>\<bbbT> CONST AgIdx_N \<lbrakk>start : len\<rwpar> T"
 
