Phi_Semantics/PhiSem_Mem_Ptr_Ar.thy
@@ -1,0 +1,5 @@
+theory PhiSem_Mem_Ptr_Ar
+  imports PhiSem_Mem_C_Ag_Ar
+begin
+
+end
